Type subtitution for subcapturing and subtyping

CC/Subst.lean
@@ -9,6 +9,7 @@ import CC.Typed
 import CC.Subtype
 import CC.Term
 import CC.Typed.Rename
+import CC.Subtype.Rename
 
 namespace CC
 
@@ -17,6 +18,9 @@ def VarSubst (Γ : Ctx n1 m) (Δ : Ctx n2 m) (f : VarMap n1 n2) : Prop :=
 
 def TVarSubst (Γ : Ctx n m1) (Δ : Ctx n m2) (g : TypeMap n m1 m2) : Prop :=
   ∀ {X S}, BoundTVar Γ X S -> SubtypeP Δ (g X) (S.tsubst g)
+
+def VarTypeMap (Γ : Ctx n m1) (Δ : Ctx n m2) (g : TypeMap n m1 m2) : Prop :=
+  ∀ {x T}, BoundVar Γ x T -> BoundVar Δ x (T.tsubst g)
 
 theorem Typed.var_bound_type :
   BoundVar Γ x T ->
@@ -56,6 +60,65 @@ def VarSubst.ext_var (σ : VarSubst Γ Δ f) P :
     have h' := σ h
     have h'' := h'.weaken_var (P.rename f id)
     exact h''
+
+def VarTypeMap.ext_var 
+  (σ : VarTypeMap Γ Δ g) T :
+  VarTypeMap (Ctx.extend_var Γ T) (Ctx.extend_var Δ (T.tsubst g)) g.ext_var := by
+  intros x T h
+  cases h
+  case here => 
+    rw [CType.tsubst_weaken_var_comm]
+    constructor
+  case there_var =>
+    rw [CType.tsubst_weaken_var_comm]
+    constructor
+    apply σ
+    trivial
+
+def VarTypeMap.ext_tvar
+  (σ : VarTypeMap Γ Δ g) S :
+  VarTypeMap (Ctx.extend_tvar Γ S) (Ctx.extend_tvar Δ (S.tsubst g)) g.ext_tvar := by
+  intros X S h
+  cases h
+  case there_tvar =>
+    rw [CType.tsubst_weaken_tvar_comm]
+    constructor
+    apply σ
+    trivial
+
+def TVarSubst.ext_var
+  (δ : TVarSubst Γ Δ g) P :
+  TVarSubst (Ctx.extend_var Γ P) (Ctx.extend_var Δ (P.tsubst g)) g.ext_var := by
+  intros X S h
+  cases h
+  case there_var h0 =>
+    conv =>
+      arg 2
+      simp [TypeMap.ext_var]
+    rw [PType.tsubst_weaken_var_comm]
+    apply SubtypeP.weaken_var
+    apply δ
+    trivial
+
+def TVarSubst.ext_tvar
+  (δ : TVarSubst Γ Δ g) S :
+  TVarSubst (Ctx.extend_tvar Γ S) (Ctx.extend_tvar Δ (S.tsubst g)) g.ext_tvar := by
+  intros X S h
+  cases h
+  case here =>
+    conv =>
+      arg 2
+      simp [TypeMap.ext_tvar]
+    rw [PType.tsubst_weaken_tvar_comm]
+    apply SubtypeP.tvar
+    constructor
+  case there_tvar =>
+    conv =>
+      arg 2
+      simp [TypeMap.ext_tvar]
+    rw [PType.tsubst_weaken_tvar_comm]
+    apply SubtypeP.weaken_tvar
+    apply δ; trivial
 
 def VarSubst.ext_tvar (σ : VarSubst Γ Δ f) R :
   VarSubst (Ctx.extend_tvar Γ R) (Ctx.extend_tvar Δ (R.rename f id)) f := by
