CC/Subcapt/TypeSubst.lean
@@ -1,0 +1,34 @@
+import Mathlib.Data.Fin.Basic
+import CC.Basic
+import CC.Rename
+import CC.CaptureSet
+import CC.Type
+import CC.Type.TypeSubst
+import CC.Context
+import CC.TypeMap
+import CC.Subst
+import CC.Narrowing
+
+namespace CC
+
+def Subcapt.tsubst
+  (h : Subcapt Γ C1 C2)
+  (δ : VarTypeMap Γ Δ g) :
+  Subcapt Δ C1 C2 := by
+  induction h
+  case sc_trans =>
+    rename_i ih1 ih2
+    apply Subcapt.sc_trans
+    apply ih1; trivial
+    apply ih2; trivial
+  case sc_elem he =>
+    apply Subcapt.sc_elem; trivial
+  case sc_var hb =>
+    apply Subcapt.sc_var
+    have h1 := δ hb
+    simp [CType.tsubst] at h1
+    exact h1
+  case sc_set ih =>
+    apply Subcapt.sc_set
+    intros x he
+    apply ih <;> trivial
