CC/Subtype/TypeSubst.lean
@@ -1,0 +1,100 @@
+import Mathlib.Data.Fin.Basic
+import CC.Basic
+import CC.Rename
+import CC.CaptureSet
+import CC.Type
+import CC.Type.TypeSubst
+import CC.Context
+import CC.TypeMap
+import CC.Subst
+import CC.Typed
+import CC.Typed.Basic
+import CC.Subtype
+import CC.Narrowing
+import CC.Subcapt.TypeSubst
+
+namespace CC
+
+private def tsubst_motive (Γ : Ctx n m1) (S1 S2 : PType n m1) : Prop :=
+  ∀ {m2} {f : TypeMap n m1 m2} {Δ : Ctx n m2},
+    VarTypeMap Γ Δ f →
+    TVarSubst Γ Δ f →
+    SubtypeP Δ (S1.tsubst f) (S2.tsubst f)
+
+private def tsubst_motive_ctype (Γ : Ctx n m1) (S1 S2 : CType n m1) : Prop :=
+  ∀ {m2} {f : TypeMap n m1 m2} {Δ : Ctx n m2},
+    VarTypeMap Γ Δ f →
+    TVarSubst Γ Δ f →
+    Subtype Δ (S1.tsubst f) (S2.tsubst f)
+
+def SubtypeP.tsubst'
+  (h : SubtypeP Γ S1 S2) :
+  tsubst_motive Γ S1 S2 := by
+  apply SubtypeP.rec
+    (motive_1 := fun Γ T1 T2 _ => tsubst_motive_ctype Γ T1 T2)
+    (motive_2 := fun Γ S1 S2 _ => tsubst_motive Γ S1 S2)
+    <;> try (solve | trivial | aesop)
+  case capt =>
+    unfold tsubst_motive at *
+    unfold tsubst_motive_ctype at *
+    intros
+    constructor <;> try trivial
+    apply Subcapt.tsubst <;> trivial
+    rename_i ih _ _ _ _ _
+    apply ih <;> trivial
+  case refl =>
+    unfold tsubst_motive; intros
+    apply SubtypeP.refl
+  case trans =>
+    unfold tsubst_motive; intros
+    apply SubtypeP.trans <;> aesop
+  case top =>
+    unfold tsubst_motive; intros
+    simp [PType.tsubst]
+    apply SubtypeP.top
+  case tvar =>
+    unfold tsubst_motive; intros
+    simp [PType.tsubst]
+    rename_i δ
+    apply δ; trivial
+  case arr =>
+    unfold tsubst_motive_ctype; unfold tsubst_motive; intros
+    simp
+    rename_i ih1 ih2 _ f Δ σ δ
+    apply SubtypeP.arr
+    apply ih1 <;> trivial
+    apply ih2
+    apply VarTypeMap.ext_var; trivial
+    apply TVarSubst.ext_var; trivial
+  case tarr =>
+    unfold tsubst_motive_ctype; unfold tsubst_motive; intros
+    simp
+    rename_i ih1 ih2 _ f Δ σ δ
+    apply SubtypeP.tarr
+    apply ih1 <;> trivial
+    apply ih2
+    apply VarTypeMap.ext_tvar; trivial
+    apply TVarSubst.ext_tvar; trivial
+  case boxed =>
+    unfold tsubst_motive_ctype; unfold tsubst_motive; intros
+    simp
+    rename_i ih _ f Δ σ δ
+    apply SubtypeP.boxed
+    apply ih <;> trivial
+
+def SubtypeP.subst
+  (h : SubtypeP Γ S1 S2)
+  (σ : VarTypeMap Γ Δ g)
+  (δ : TVarSubst Γ Δ g) :
+  SubtypeP Δ (S1.tsubst g) (S2.tsubst g) := by
+  apply SubtypeP.tsubst' <;> aesop
+
+def Subtype.subst
+  (h : Subtype Γ T1 T2)
+  (σ : VarTypeMap Γ Δ g)
+  (δ : TVarSubst Γ Δ g) :
+  Subtype Δ (T1.tsubst g) (T2.tsubst g) := by
+  cases h
+  constructor
+  apply Subcapt.tsubst <;> trivial
+  apply SubtypeP.subst <;> trivial
